yet another approach

theories/examples/syntax/syntax.sig
@@ -1,6 +1,3 @@
-nat : Type
-
-
 Tm(var) : Type 
 abs     : Tm -> (bind Tm in Tm) -> Tm
 app     : Tm -> Tm -> Tm
@@ -9,6 +6,6 @@ succ    : Tm -> Tm
 nrec    : (bind Tm in Tm) -> Tm -> Tm -> Tm
 tnat    : Tm
 tpi     : Tm -> (bind Tm in Tm) -> Tm
-tuniv   : nat -> Tm   
+tuniv   : Tm   
 
 
