theories/examples/finelt/raw_validity2.v
@@ -17,6 +17,7 @@ Require Import syntax.typing.
 Require Import syntax.relations.
 
 
+
 Import SyntaxNotations.
 Import SubstNotations.
 
@@ -71,27 +72,23 @@ Qed.
 
 Require Import findom.
 Require Import types.
-Require Import raw_semantics.
-Require Import typing_semantics.
-Require Import eval_substitution.
-
 
 Import Raw.
-    
+
 
 (*
 (* Inversion lemmas for wt *)
 Lemma wt_tpi_dom (a : elt) (g : list (elt * elt)) (j : nat):
-  wt (tpi a g) (tuniv j) ->
-  wt a (tuniv j).
+  wt (tpi a g) tuniv ->
+  wt a tuniv.
 move=>h. inversion h. done. Defined.
 Lemma wt_tpi_cod_key (a : elt) (g : list (elt * elt)) (j : nat):
-  wt (tpi a g) (tuniv j) ->
+  wt (tpi a g) tuniv ->
   (forall ui vi : elt, In (ui, vi) g -> wt ui a).
 move=>h. inversion h. done. Defined.
 Lemma wt_tpi_cod_elt (a : elt) (g : list (elt * elt)) (j : nat):
-  wt (tpi a g) (tuniv j) ->
-  (forall ui vi : elt, In (ui, vi) g -> wt vi (tuniv j)).
+  wt (tpi a g) tuniv ->
+  (forall ui vi : elt, In (ui, vi) g -> wt vi tuniv).
 move=>h. inversion h. done. Defined.
 *)
 
@@ -102,14 +99,14 @@ move=>h. inversion h. done. Defined.
  *)
 (*
 Lemma wt_abs_dom f a g : 
-  wt (abs f) (tpi a g) -> { i & wt a (tuniv i) }.
+  wt (abs f) (tpi a g) -> { i & wt a tuniv }.
 Proof.
 move=> h. inversion h. subst.
 inversion H4. subst. eexists. eauto.
 Qed.
 
 Lemma wt_abs_tpi f a g : 
-  wt (abs f) (tpi a g) -> { i &  wt (tpi a g) (tuniv i) }.
+  wt (abs f) (tpi a g) -> { i &  wt (tpi a g) tuniv }.
 move=> h. inversion h. subst. eexists. eauto.
 Qed.
 *)
@@ -151,6 +148,50 @@ Admitted.
 
 
 
+Lemma wt_abs_ty g b f : 
+  wt (abs g) (tpi b f) -> wt (tpi b f) tuniv.
+Proof. 
+  move=> h. inversion h. eauto.
+Defined.
+
+
+Lemma wt_abs_inv1 g a f : 
+  wt (abs f) (tpi a g) ->     
+  (forall u v, valid u -> app f u = Some v -> ~ is_bot v -> wt u a).
+Proof. 
+  move=> h. inversion h. eauto.
+Defined.
+
+Lemma wt_abs_inv2 g a f : 
+  wt (abs f) (tpi a g) ->    
+  (forall u v t, valid u -> app f u = Some v -> ~ is_bot v -> app g u = Some t -> wt v t). 
+Proof. 
+  move=> h. inversion h. eauto.
+Defined.
+
+
+Lemma wt_tpi_dom a g :
+  wt (tpi a g) tuniv  -> wt a tuniv.
+Proof.
+  move=> h. inversion h. eauto.
+Defined.
+
+
+Lemma wt_tpi_inv1 a g :
+  wt (tpi a g) tuniv -> 
+  (forall u v, valid u -> app g u = Some v -> ~ is_bot v -> wt u a).
+Proof.
+  move=> h. inversion h. eauto.
+Defined.
+
+Lemma wt_tpi_inv2 a g :
+  wt (tpi a g) tuniv -> 
+  (forall u v, valid u -> app g u = Some v -> ~ is_bot v -> wt v tuniv).
+Proof.
+  move=> h. inversion h. eauto.
+Defined.
+
+
 (* This module defines various helper operations on the logical
    relation. Each of these operations is parameterized by the
    two main fixpoints (Val and EqVal) which are polymorphic in
@@ -160,220 +201,233 @@ Module Rec.
 
 Record F := MkF {
    Val   : forall {n} (Γ : Ctx n),
-              Tm n -> Tm n -> forall u a, wt u a -> forall i, wt a (tuniv i) -> Prop;
+              Tm n -> Tm n -> forall u a, wt u a -> Prop;
    EqVal : forall {n} (Γ : Ctx n),
-              Tm n -> Tm n -> Tm n -> forall u a, wt u a -> forall i, wt a (tuniv i) -> Prop;
+              Tm n -> Tm n -> Tm n -> forall u a, wt u a -> Prop;
+(*
    PiEdgeVal : forall {n} (Γ : Ctx n)
      (A : Tm n) (B : Tm (S n)) (b: elt) (f : list (elt * elt))
-     i (h : wt_pi_fun f b i), Prop ;
+     (h1 : wt (tpi b f) tuniv), Prop ; 
    PiEdgeEq  : forall {n} (Γ : Ctx n)
                  (A : Tm n) (B : Tm (S n)) (b: elt)
                  (f : list (elt * elt))
-                 i (h : wt_pi_fun f b i), Prop;
+                 (h1 : wt (tpi b f) tuniv), Prop;
    PiEdgeEqTy: forall {n} (Γ : Ctx n) (A:Tm n) (B B': Tm (S n))
-                 b f i (h : wt_pi_fun f b i), Prop;
+                 (b: elt) (f: list (elt * elt)) 
+                 (h: wt (tpi b f) tuniv), Prop;
    PiAppVal: forall {n} (Γ : Ctx n)
      (M : Tm n) (A0 : Tm n) (B0 : Tm (S n)) b f g
-     (h1 : wt_abs_fun g b f)
-     i (h2 : wt_pi_fun f b i), Prop;
+     (h1 : wt (abs g) (tpi b f))
+     , Prop;
    PiAppEq :forall {n} (Γ : Ctx n)
-  (M : Tm n) (A0 : Tm n) (B0 : Tm (S n)) b f g
-  (h1 : wt_abs_fun g b f)
-  i (h2 : wt_pi_fun f b i), Prop;
+              (M : Tm n) (A0 : Tm n) (B0 : Tm (S n)) b f g
+              (h1 : wt (abs g) (tpi b f))
+                , Prop;
 PiAppEqVal : forall {n} (Γ : Ctx n)
   (M N : Tm n) (A0 : Tm n) (B0 : Tm (S n)) b f g
-  (h : wt_abs_fun g b f) i (h2 : wt_pi_fun f b i), Prop
+  (h : wt (abs g) (tpi b f)) , Prop *)
 }.
+
 
 
 Section Helpers.
 
-(*
-Inductive wt : elt -> elt -> Set :=
-    wt_bot : forall (a : elt) (i : nat), wt a (tuniv i) -> wt bot a
-  | wt_tuniv : forall i j : nat, i < j -> wt (tuniv i) (tuniv j)
-  | wt_tnat : forall j : nat, wt tnat (tuniv j)
-  | wt_zero : wt zero tnat
-  | wt_succ : forall u : elt, wt u tnat -> wt (succ u) tnat
-  | wt_tpi : forall (a : elt) (g : list (elt * elt)) (j : nat),
-             wt_pi_fun g a j -> wt a (tuniv j) -> valid (tpi a g) -> wt (tpi a g) (tuniv j)
-  | wt_abs : forall (a : elt) (f g : list (elt * elt)) (i : nat),
-             wt_abs_fun f a g -> valid (abs f) -> wt (tpi a g) (tuniv i) -> wt (abs f) (tpi a g)
-  with wt_pi_fun : list (elt * elt) -> elt -> nat -> Set :=
-    wt_pi_nil : forall (a : elt) (i : nat), wt_pi_fun nil a i
-  | wt_pi_cons : forall (a ui vi : elt) (g : list (elt * elt)) (i : nat),
-                 wt ui a -> wt vi (tuniv i) -> wt_pi_fun g a i -> wt_pi_fun ((ui, vi) :: g) a i
-  with wt_abs_fun : list (elt * elt) -> elt -> list (elt * elt) -> Set :=
-    wt_abs_nil : forall (a : elt) (g : list (elt * elt)), wt_abs_fun nil a g
-  | wt_abs_cons : forall (ui vi : elt) (f : list (elt * elt)) (a : elt) (g : list (elt * elt))
-                    (t : elt),
-                  wt ui a ->
-                  app g ui = Some t -> wt vi t -> wt_abs_fun f a g -> wt_abs_fun ((ui, vi) :: f) a g.
-*)
-
 Variable (Rec : F).
-(*
-  (Val   : forall {n} (Γ : Ctx n),
-              Tm n -> Tm n -> forall u a, wt u a -> Prop)
-  (EqVal : forall {n} (Γ : Ctx n),
-              Tm n -> Tm n -> Tm n -> forall u a, wt u a -> Prop)
-  (PiEdgeVal : forall {n} (Γ : Ctx n)
-     (A : Tm n) (B : Tm (S n)) (b: elt) (f : list (elt * elt))
-     i (h : wt_pi_fun f b i), Prop)
-  (PiEdgeEq  : forall {n} (Γ : Ctx n)
-                 (A : Tm n) (B : Tm (S n)) (b: elt) (f : list (elt * elt))
-                 i (h : wt_pi_fun f b i), Prop)
-  (PiEdgeEqTy: forall {n} (Γ : Ctx n) A B B' b f i (h : wt_pi_fun b f i), Prop).
-*)
 
-(*
-Fixpoint PiEdgeVal {n} (Γ : Ctx n)
+
+
+Definition  PiEdgeEq {n} (Γ : Ctx n)
   (A : Tm n) (B : Tm (S n)) (b: elt) (f : list (elt * elt))
-  i (h : wt_pi_fun f b i) : Prop :=
-  match h with 
-  | wt_pi_nil _ _ => True
-  | @wt_pi_cons a ui vi g i WTui WTvi WTf => 
-      PiEdgeVal Γ A B WTf /\
-      forall (N : Tm n),
-        typing Γ N A ->
-        (* take related arguments *)
-        Val Γ N A WTui ->
-        (* to related results *)
-        Val Γ B[N..] (Core.tuniv i) WTvi  
-  end.
-*)
+  (h : wt (tpi b f) tuniv) :=
+  forall u v (Vu : valid u) 
+      (APP: app f u = Some v) (NB: ~ is_bot v) 
+      (N1 N2 : Tm n),
+      conv Γ N1 N2 A ->
+      (* take related arguments *)
+      EqVal Rec Γ N1 N2 A (wt_tpi_inv1 h Vu APP NB) ->
+      (* to related results *)
+      EqVal Rec Γ B[N1..] B[N2..] Core.tuniv (wt_tpi_inv2 h Vu APP NB).
 
+Definition PiAppVal {n} (Γ : Ctx n)
+  (M : Tm n) (A0 : Tm n) (B0 : Tm (S n)) b f g
+  (h : wt (abs f) (tpi b g)) : Prop :=
+  forall u v t (Vu : valid u) 
+  (APP: app f u = Some v) (NB: ~ is_bot v) 
+  (APPg : app g u = Some t)
+  (P : Tm n), typing Γ P A0 -> 
+              Val Rec Γ P A0 (wt_abs_inv1 h Vu APP NB) -> 
+              Val Rec Γ (Core.app M P) B0[P..] 
+                  (wt_abs_inv2 h Vu APP NB APPg). 
 
-
-
-Lemma wt_abs_inv g b f : 
-  wt (abs g) (tpi b f) -> wt_abs_fun g b f.
-Proof. 
-  move=> h. inversion h. eauto.
-Defined.
-
-Lemma wt_tpi_dom a g i:
-  wt (tpi a g) (tuniv i) -> wt a (tuniv i).
-Proof.
-  move=> h. inversion h. eauto.
-Defined.
-
-Lemma wt_tpi_inv a g i:
-  wt (tpi a g) (tuniv i) -> wt_pi_fun g a i.
-Proof.
-  move=> h. inversion h. eauto.
-Defined.
+Definition PiAppEq {n} (Γ : Ctx n)
+  (M : Tm n) (A0 : Tm n) (B0 : Tm (S n)) b f g
+  (h : wt (abs f) (tpi b g))  := 
+  forall u v t (Vu : valid u) 
+    (APP: app f u = Some v) (NB: ~ is_bot v) 
+    (APPg : app g u = Some t)
+    (N1 N2 : Tm n),
+    conv Γ N1 N2 A0 ->
+    EqVal Rec Γ N1 N2 A0 (wt_abs_inv1 h Vu APP NB) ->
+    EqVal Rec Γ (Core.app M N1) (Core.app M N2) B0[N1..] 
+          (wt_abs_inv2 h Vu APP NB APPg).
+    
+Definition PiAppEqVal {n} (Γ : Ctx n)
+  (M N : Tm n) (A0 : Tm n) (B0 : Tm (S n)) b f g
+  (h : wt (abs f) (tpi b g)) :=
+  forall  u v t (Vu : valid u) 
+  (APP: app f u = Some v) (NB: ~ is_bot v) 
+  (APPg : app g u = Some t) (P : Tm n),
+        typing Γ P A0 ->
+        Val Rec Γ P A0 (wt_abs_inv1 h Vu APP NB) ->
+        EqVal Rec Γ (Core.app M P) (Core.app N P) B0[P..]
+          (wt_abs_inv2 h Vu APP NB APPg).
 
 Definition ValPi {n} (Γ : Ctx n)
-  (M : Tm n) (A : Tm n) g b f (h : wt (abs g) (tpi b f))
-  i (h2 : wt (tpi b f) (tuniv i)):=
+  (M : Tm n) (A : Tm n) g b f (h : wt (abs g) (tpi b f)):=
   exists A0, exists B0, HeadRed A (Core.tpi A0 B0)
-  /\ PiAppVal Rec Γ M A0 B0 (wt_abs_inv h) (wt_tpi_inv h2) .
+  /\ PiAppVal Γ M A0 B0 h.
 
 Definition EqValPi {n} (Γ : Ctx n)
   (M : Tm n) (N: Tm n) (A : Tm n) g b f 
-  (h : wt (abs g) (tpi b f)) i (h2 : wt (tpi b f) (tuniv i)) :=
+  (h : wt (abs g) (tpi b f)) :=
   exists A0, exists B0, HeadRed A (Core.tpi A0 B0)
-  /\ 
-    PiAppEqVal Rec Γ M N A0 B0 (wt_abs_inv h) (wt_tpi_inv h2).
+  /\ PiAppEqVal Γ M N A0 B0 h.
 
-Definition ValTy {n} (Γ : Ctx n)
-  (M : Tm n) u i : wt u (tuniv i) -> forall j, wt (tuniv i) (tuniv j) -> Prop  :=
-  match u return wt _ (tuniv i) -> forall j, wt (tuniv i) (tuniv j) -> Prop with
+
+
+Fixpoint ValTy {n} (Γ : Ctx n)
+  (M : Tm n) u (h : wt u tuniv) {struct h} : Prop  :=
+
+  let PiEdgeVal {n} (Γ : Ctx n)
+        (A : Tm n) (B : Tm (S n)) (b: elt) (f : list (elt * elt))
+        (h : wt (tpi b f) tuniv) : Prop := 
+    forall u v (Vu : valid u) 
+        (APP: app f u = Some v) (NB: ~ is_bot v) (WTu : wt u b)
+        (N : Tm n), typing Γ N A ->
+                    (* take related arguments *)
+                    Val Rec Γ N A (wt_tpi_inv1 h Vu APP NB) ->
+                    (* to related results *)
+                    ValTy Γ B[N..] (wt_tpi_inv2 h Vu APP NB)
+  in
+
+  (match u return wt _ tuniv ->  Prop with
   | tpi b g =>
-      fun (h : wt (tpi b g) (tuniv i)) j (h2 : wt (tuniv i) (tuniv j)) =>
-        (* ValTyPi M (tuniv i) *)
+      fun (h : wt (tpi b g) tuniv) =>
+        (* ValTyPi M tuniv *)
         (* M reduces to a pi type *)
         exists A B, HeadRed M (Core.tpi A B)
 
                (* the syntactic pi-type is well-typed *)              
-               /\ typing Γ A (Core.tuniv i)
-               /\ typing (Γ ++ A) B (Core.tuniv i)
-               
+               /\ typing Γ A Core.tuniv
+               /\ typing (Γ ++ A) B Core.tuniv
 
                (* the semantic pi-type is valid *)
                /\ valid (tpi b g)
 
-               (* domain is in the relation *)
-               /\ Val Rec Γ A (Core.tuniv i) (wt_tpi_dom h)
-                                            h2
-               /\ PiEdgeVal Rec Γ A B (wt_tpi_inv h) 
-               /\ PiEdgeEq Rec Γ A B (wt_tpi_inv h)
+               (* domain (b) is in the relation *)
+               /\ Val Rec Γ A Core.tuniv (wt_tpi_dom h)
+                                          
+               /\ PiEdgeVal Γ A B b g h 
+               /\ PiEdgeEq Γ A B h
 
-  | tnat => fun h1 j h2 => True
-  | tuniv k => fun h1 j h2 => True
-  | _ => fun h1 j h2 => True
-  end.
+  | tnat => fun h1 => True
+  | tuniv => fun h1  => True
+  | _ => fun h1  => True
+  end) h.
 
-Definition EqValTy {n} (Γ : Ctx n) M N (a : elt) i (h : wt a (tuniv i)) :  forall j, wt (tuniv i) (tuniv j) -> Prop :=
-  (match a return wt _ (tuniv i) ->  forall j, wt (tuniv i) (tuniv j) -> Prop with
+
+(*  match h with 
+  | wt_pi_nil _ => True
+  | @wt_pi_cons a ui vi g WTui WTvi WTf Vg => 
+      PiEdgeEqTy Γ A B B' WTf /\
+        forall (P : Tm n),
+          typing Γ P A ->
+          (* take related arguments *)
+          Val Γ P A WTui ->
+          (* to related results *)
+          Rec.EqValTy Rec Γ B[P..] B'[P..] WTvi
+  end *)
+
+
+Fixpoint EqValTy {n} (Γ : Ctx n) M N (a : elt) (h : wt a tuniv) {struct h} :  Prop :=
+  let PiEdgeEqTy {n} (Γ : Ctx n) 
+  (A : Tm n) (B B' : Tm (S n)) b f (h : wt (tpi b f) tuniv)  := 
+    forall u v (Vu : valid u) 
+      (APP: app f u = Some v) (NB: ~ is_bot v) 
+      (P : Tm n),
+          typing Γ P A ->
+          (* take related arguments *)
+          Val Rec Γ P A (wt_tpi_inv1 h Vu APP NB) ->
+          (* to related results *)
+          EqValTy Γ B[P..] B'[P..] (wt_tpi_inv2 h Vu APP NB)
+  in 
+  (match a return wt _ tuniv ->  Prop with
   | tpi b f =>
-      fun (h : wt (tpi b f) (tuniv i)) j h2  =>
-        ValTy Γ M h h2 /\ ValTy Γ N h h2 /\
+      fun (h : wt (tpi b f) tuniv)  =>
+        ValTy Γ M h  /\ ValTy Γ N h /\
         (* EqValTyPi Val EqVal EqValTy M N h *)
              (* both reduce to pi types *)
              exists A B, HeadRed M (Core.tpi A B)
              /\ exists A' B', HeadRed N (Core.tpi A' B')
              (* ... that are convertible *)
-             /\ conv Γ A A' (Core.tuniv i)
-             /\ conv (Γ ++ A) B B' (Core.tuniv i) 
+             /\ conv Γ A A' Core.tuniv 
+             /\ conv (Γ ++ A) B B' Core.tuniv 
              /\ valid (tpi b f)
              (* ... and the domain is in the relation *)
-             /\ EqVal Rec Γ A A' (Core.tuniv i) (wt_tpi_dom h) h2
-             /\ PiEdgeEqTy Rec Γ A B B' (wt_tpi_inv h)
-  | _ => fun h j h2 => True
+             /\ EqVal Rec Γ A A' Core.tuniv  (wt_tpi_dom h) 
+             /\ PiEdgeEqTy Γ A B B' _ _ h
+  | _ => fun h => True
   end) h.
+
+
 
 End Helpers.
 End Rec.
 
 Fixpoint Val {n} (Γ : Ctx n)
-  (M : Tm n) (A : Tm n) (u : elt) (a: elt) (h : wt u a) i (h2 : wt a (tuniv i)) { struct h } : Prop :=
-  let Rec := Rec.MkF (@Val) (@EqVal) (@PiEdgeVal) (@PiEdgeEq) (@PiEdgeEqTy)
-  (@PiAppVal) (@PiAppEq) (@PiAppEqVal) in
-      (match a return wt u _ -> forall j, wt _ (tuniv j) -> Prop with
+  (M : Tm n) (A : Tm n) (u : elt) (a: elt) (h : wt u a)  
+  { struct h } : Prop :=
+  let Rec := Rec.MkF (@Val) (@EqVal) in
+      (match a return wt u _ -> Prop with
 
-      | bot => fun h j h2 => True
+      | bot => fun h => True
 
-      | tuniv i => fun (h : wt u (tuniv i)) j h2 =>
-          Rec.ValTy Rec Γ M h h2
+      | tuniv => fun (h : wt u tuniv) =>
+          Rec.ValTy Rec Γ M h 
 
-      | tpi b f => fun h j h2 =>
-           (match u return wt _ (tpi b f) ->  forall j, wt (tpi b f) (tuniv j) -> Prop with
+      | tpi b f => fun h  =>
+           (match u return wt _ (tpi b f) ->  Prop with
 
-            | abs g => fun (h : wt (abs g) (tpi b f)) j h2 =>
-                        match h with 
-                        | wt_abs WTf Vf Vtpi =>
-                            Rec.ValTy Rec Γ A h2 (@wt_tuniv j (S j) ltac:(lia))
-                        | _ => True
-                        end
-                        
-                      /\ Rec.ValPi Rec Γ M A h h2
+            | abs g => fun (h : wt (abs g) (tpi b f)) =>
+    (*    Pair (ValTy2 G A (PiCode b f)) (ValPi2 G M A g b f) *)
+                      Rec.ValTy Rec Γ A (wt_abs_ty h)
+                      /\ Rec.ValPi Rec Γ M A h 
 
-            | _ => fun h j h2 => True
-            end) h j h2
+            | _ => fun h  => True
+            end) h 
 
-      | tnat => fun h j h2 =>
-          (match u return wt _ tnat ->  forall j, wt _ (tuniv j) -> Prop with
-               | zero => fun h j h2 =>
+      | tnat => fun h =>
+          (match u return wt _ tnat -> Prop with
+               | zero => fun h  =>
                  HeadRed M (Core.zero)
-               | succ v => fun (h : wt (succ v) tnat) j h2 =>
+               | succ v => fun (h : wt (succ v) tnat)  =>
                  exists M1, HeadRed M (Core.succ M1)
-                 /\ Val Γ M1 Core.tnat (wt_succ_inv h) h2
-               | _ =>  fun h j h2 => True
-               end) h j h2
-      | _ => fun h j h2 => True
-    end) h i h2
+                 /\ Val Γ M1 Core.tnat (wt_succ_inv h) 
+               | _ =>  fun h => True
+               end) h
+      | _ => fun h  => True
+    end) h 
 (* Binary logical relation *)
 with EqVal {n} (Γ : Ctx n)
-  (M : Tm n) (N : Tm n) (A : Tm n) (u : elt) (a: elt) (h : wt u a) i (h2 : wt a (tuniv i)) { struct h } : Prop :=
-  let Rec := Rec.MkF (@Val) (@EqVal) (@PiEdgeVal) (@PiEdgeEq) (@PiEdgeEqTy)(@PiAppVal) (@PiAppEq) (@PiAppEqVal) in
+  (M : Tm n) (N : Tm n) (A : Tm n) (u : elt) (a: elt) (h : wt u a) 
+  { struct h } : Prop :=
+  let Rec := Rec.MkF (@Val) (@EqVal)  in
        
      (match a return wt u _ -> Prop with
 
       | bot => fun h => True
 
-      | tuniv i => fun (h : wt u (tuniv i)) =>
+      | tuniv => fun (h : wt u tuniv) =>
 
             Rec.ValTy Rec Γ M h
           /\ Rec.ValTy Rec Γ N h
@@ -383,11 +437,7 @@ with EqVal {n} (Γ : Ctx n)
            (match u return wt _ (tpi b f) -> Prop with
            | bot => fun h => True
            | abs g => fun (h : wt (abs g) (tpi b f)) =>
-              match h with 
-              | wt_abs WTf Vf (wt_tpi _ WTa _) =>
-                  Rec.ValTy Rec Γ A WTa
-              | _ => True
-              end
+               Rec.ValTy Rec Γ A (wt_abs_ty h)
              /\ Rec.ValPi Rec Γ M A h
              /\ Rec.ValPi Rec Γ N A h
              /\ Rec.EqValPi Rec Γ M N A h
@@ -407,114 +457,17 @@ with EqVal {n} (Γ : Ctx n)
                | _ =>  fun h => True
                end) h
       | _ => fun h => True
-    end) h
-with 
- PiEdgeVal {n} (Γ : Ctx n)
-  (A : Tm n) (B : Tm (S n)) (b: elt) (f : list (elt * elt))
-  i (h : wt_pi_fun f b i) {struct h} : Prop :=
-  let Rec := Rec.MkF (@Val) (@EqVal) (@PiEdgeVal) (@PiEdgeEq) (@PiEdgeEqTy)(@PiAppVal) (@PiAppEq) (@PiAppEqVal) in
-
-  match h with 
-  | wt_pi_nil _ _ => True
-  | @wt_pi_cons a ui vi g i WTui WTvi WTf => 
-      PiEdgeVal Γ A B WTf /\
-      forall (N : Tm n),
-        typing Γ N A ->
-        (* take related arguments *)
-        Val Γ N A WTui ->
-        (* to related results *)
-        Val Γ B[N..] (Core.tuniv i) WTvi  
-  end
-with
-  PiEdgeEq {n} (Γ : Ctx n)
-  (A : Tm n) (B : Tm (S n)) (b: elt) (f : list (elt * elt))
-  i (h : wt_pi_fun f b i) {struct h} :=
-
-  match h with 
-  | wt_pi_nil _ _ => True
-  | @wt_pi_cons a ui vi g i WTui WTvi WTf => 
-      PiEdgeEq Γ A B WTf /\
-      forall (N1 N2 : Tm n),
-      conv Γ N1 N2 A ->
-      (* take related arguments *)
-      EqVal Γ N1 N2 A WTui ->
-      (* to related results *)
-      EqVal Γ B[N1..] B[N2..] (Core.tuniv i) WTvi
-  end
-with
-  PiEdgeEqTy {n} (Γ : Ctx n) A B B' b f i (h : wt_pi_fun f b i)            
-    {struct h} := 
-  let Rec := Rec.MkF (@Val) (@EqVal) (@PiEdgeVal) (@PiEdgeEq) (@PiEdgeEqTy)(@PiAppVal) (@PiAppEq) (@PiAppEqVal) in
-
-  match h with 
-  | wt_pi_nil _ _ => True
-  | @wt_pi_cons a ui vi g i WTui WTvi WTf => 
-      PiEdgeEqTy Γ A B B' WTf /\
-        forall (P : Tm n),
-          typing Γ P A ->
-          (* take related arguments *)
-          Val Γ P A WTui ->
-          (* to related results *)
-          Rec.EqValTy Rec Γ B[P..] B'[P..] WTvi
-  end
-with PiAppVal {n} (Γ : Ctx n)
-  (M : Tm n) (A0 : Tm n) (B0 : Tm (S n)) b f g
-  (h : wt_abs_fun g b f) j (h2: wt_pi_fun f b j) : Prop :=
-  match h with 
-  | wt_abs_nil _ _ => True
-  | @wt_abs_cons  ui vi f a g t WTui APPu WTvi WTf => 
-      PiAppVal Γ M A0 B0 WTf /\
-      forall (P : Tm n),
-        typing Γ P A0 ->
-        Val Γ P A0 WTui ->
-        Val Γ (Core.app M P) B0[P..] WTvi
-  end
-with PiAppEq {n} (Γ : Ctx n)
-  (M : Tm n) (A0 : Tm n) (B0 : Tm (S n)) b f g
-  (h : wt_abs_fun g b f) j (h2: wt_pi_fun f b j) :=
-  match h with 
-  | wt_abs_nil _ _ => True
-  | @wt_abs_cons  ui vi f a g t WTui APPu WTvi WTf => 
-      PiAppEq Γ M A0 B0 WTf /\
-      forall (N1 N2 : Tm n),
-        conv Γ N1 N2 A0 ->
-        EqVal Γ N1 N2 A0 WTui ->
-        EqVal Γ (Core.app M N1) (Core.app M N2) B0[N1..] WTvi
-  end
-with PiAppEqVal {n} (Γ : Ctx n)
-  (M N : Tm n) (A0 : Tm n) (B0 : Tm (S n)) b f g
-  (h : wt_abs_fun g b f) j (h2: wt_pi_fun f b j) :=
-  match h with 
-  | wt_abs_nil _ _ => True
-  | @wt_abs_cons  ui vi f a g t WTui APPu WTvi WTf => 
-      PiAppEqVal Γ M N A0 B0 WTf /\
-      forall (P : Tm n),
-        typing Γ P A0 ->
-        Val Γ P A0 WTui ->
-        EqVal Γ (Core.app M P) (Core.app N P) B0[P..] WTvi
-  end.
-
-
-Notation Rec := (Rec.MkF (@Val) (@EqVal) (@PiEdgeVal) (@PiEdgeEq) (@PiEdgeEqTy)(@PiAppVal) (@PiAppEq) (@PiAppEqVal)).
+    end) h.
 
 
 
-Notation ValTy := (@Rec.ValTy Rec).
-Notation EqValTy := (@Rec.EqValTy Rec).
-Notation ValPi := (@Rec.ValPi
-      {|
-        Rec.Val := @Val;
-        Rec.EqVal := @EqVal;
-        Rec.PiEdgeVal := @PiEdgeVal;
-        Rec.PiEdgeEq := @PiEdgeEq;
-        Rec.PiEdgeEqTy := @PiEdgeEqTy;
-        Rec.PiAppVal := @PiAppVal;
-        Rec.PiAppEq := @PiAppEq;
-        Rec.PiAppEqVal := @PiAppEqVal
-      |}).
-Notation EqValPi := 
-  (@Rec.EqValPi 
-    (Rec.MkF (@Val) (@EqVal) (@PiEdgeVal) (@PiEdgeEq) (@PiEdgeEqTy)(@PiAppVal) (@PiAppEq) (@PiAppEqVal))).
+Notation Rec := (Rec.MkF (@Val) (@EqVal)). 
+
+Definition ValTy := (@Rec.ValTy Rec).
+Definition EqValTy := (@Rec.EqValTy Rec).
+Definition ValPi := (@Rec.ValPi Rec).
+Definition EqValPi := (@Rec.EqValPi Rec).
+
 
 (* All terms in the relation have the right syntactic type.
  NOT TRUE*)
@@ -528,16 +481,8 @@ Proof.
   - destruct a; try done.
 Abort.
 
-(* Incomplete stub commented out — references undefined u, b, f, h1 and has no Proof block.
-
-wt_tpi
-     : forall (a : elt) (g : list (elt * elt)) (j : nat),
-       wt_pi_fun g a j -> wt a (tuniv j) -> valid (tpi a g) -> wt (tpi a g) (tuniv j)
-
-*)
-
 (*
-Lemma EqVal_tpi n (Γ:Ctx n) M N A f g a i u b (w : wt_pi_fun g a i) (h : wt a (tuniv i)) (V : valid (tpi a g)) :
+Lemma EqVal_tpi n (Γ:Ctx n) M N A f g a i u b (w : wt_pi_fun g a i) (h : wt a tuniv) (V : valid (tpi a g)) :
   (EqVal Γ M N A (wt_tpi w h V : wt u b)) =
       (match h return wt _ (tpi a g) -> Prop with
            | bot => fun h => True
@@ -576,9 +521,9 @@ Qed.
    Val <-> ValTy  and  EqVal <-> EqValTy
    ============================================================ *)
 
-Lemma EqValTy_EqVal {n} (Γ : Ctx n) (A B : Tm n) a i (h : wt a (tuniv i)):
+Lemma EqValTy_EqVal {n} (Γ : Ctx n) (A B : Tm n) a (h : wt a tuniv):
   EqValTy Γ A B h ->
-  EqVal Γ A B (Core.tuniv i) h.
+  EqVal Γ A B Core.tuniv h.
 Proof.
   dependent destruction h; try done.
   all: cbn.
@@ -586,7 +531,7 @@ Proof.
   all: eauto.
 Qed.
 
-Lemma EqVal_EqValTy {n} (Γ : Ctx n) (A B C : Tm n) a i (h : wt a (tuniv i)):
+Lemma EqVal_EqValTy {n} (Γ : Ctx n) (A B C : Tm n) a (h : wt a tuniv):
   EqVal Γ A B C h ->
   EqValTy Γ A B h.
 Proof.
@@ -595,15 +540,15 @@ Proof.
   all: eauto.
 Qed.
 
-Lemma ValTy_Val {n} (Γ : Ctx n) (A : Tm n) a i (h : wt a (tuniv i)):
+Lemma ValTy_Val {n} (Γ : Ctx n) (A : Tm n) a (h : wt a tuniv):
   ValTy Γ A h ->
-  Val Γ A (Core.tuniv i) h.
+  Val Γ A Core.tuniv h.
 Proof.
   dependent destruction h; try done.
 Qed.
 
-Lemma Val_ValTy {n} (Γ : Ctx n) (A : Tm n) a i (h : wt a (tuniv i)):
-  Val Γ A (Core.tuniv i) h ->
+Lemma Val_ValTy {n} (Γ : Ctx n) (A : Tm n) a (h : wt a tuniv):
+  Val Γ A Core.tuniv h ->
   ValTy Γ A h.
 Proof.
   dependent destruction h; try done.
@@ -619,64 +564,63 @@ Qed.
 
 
 Fixpoint Val_EqVal {n} (Γ : Ctx n) (M A : Tm n) u a (h : wt u a) {struct h} :
-  Val Γ M A h -> EqVal Γ M M A h
-with PiEdgeEq_PiEdgeEqTy {n} (Γ : Ctx n) (A : Tm n) (B : Tm (S n)) b f i (h : wt_pi_fun b f i) {struct h} :
-  PiEdgeEq Γ A B h ->
+  Val Γ M A h -> EqVal Γ M M A h.
+(*
+with PiEdgeEq_PiEdgeEqTy {n} (Γ : Ctx n) (A : Tm n) (B : Tm (S n)) b f (h : wt_pi_fun b f) {struct h} :
+ PiEdgeEq Γ A B h ->
   PiEdgeEqTy Γ A B B h
 with PiAppVal_PiAppEqVal {n} (Γ : Ctx n) (M : Tm n) (A : Tm n) (B : Tm (S n)) b f g
   (h : wt_abs_fun g b f) {struct h} : 
   PiAppVal Γ M A B h -> 
-  PiAppEqVal Γ M M A B h.
+  PiAppEqVal Γ M M A B h. *)
 Proof.
 + dependent destruction h.
   all: cbn.
   all: eauto.
   - destruct a; try done.
-  - move=> [M1 [h1 V1]].
+  - 
+    move=> [M1 [h1 V1]].
     exists M1. split; auto.
     exists M1. split; auto.
-  - move=>h1.
+  - (* tpi *) 
+    move=>h1.
     repeat split; eauto.
     clear A.
-    destruct h1 as (A & B & HR & (* TA & TB & *) VPi & ValA & PEV & PEE).
+    destruct h1 as (A & B & HR &  TA & TB & VPi & ValA & PEV & PEE).
     exists A, B. split; auto.
     exists A, B. split; auto.
-(*    repeat split; auto.
+    repeat split; auto.
     eapply c_refl; eauto.
-    eapply c_refl; eauto. *)
-  - move=> h1.
+    eapply c_refl; eauto. 
+    move=> u v Vu APP NB P TP VA.
+    unfold Rec.PiEdgeEq in PEE.
+    specialize (PEV u v Vu APP NB).
+    specialize (PEE u v Vu APP NB).
+    eapply EqVal_EqValTy.
+    eapply PEE.
+    eapply c_refl; eauto.
+    cbn.
+    eapply Val_EqVal. eapply VA.
+  - (* abs *)
+    move=> [HR PAV].
+    inversion h. subst.
     repeat split; eauto.
-    destruct h1 as (HR & PAV).
-    dependent destruction h.
     unfold Rec.ValPi in PAV.
     destruct PAV as [A0 [B0 [R1 PAV]]].
     unfold Rec.EqValPi.
     exists A0, B0. split; eauto.
     unfold Rec.PiAppEqVal.
     unfold Rec.PiAppVal in PAV.
-    eauto.
-+ (* EdgeEq *)
-  dependent destruction h.
-  - done.
-  - move=> PEE. cbn in PEE.
-    move: PEE => [PEE h1].
-    cbn. split. eauto.
-    move=> P TP VP.
-    eapply EqVal_EqValTy.
-    eapply h1; eauto.
-    eapply c_refl. auto.
-+ dependent destruction h.
-  - done.
-  - move=> PAV. cbn in PAV.
-    move: PAV => [PAV h1].
-    cbn. split. eauto.
-    move=> P TP VP.
-    eapply Val_EqVal. eapply h1; eauto.
-Qed.
+    move=> u v t Vu APP NB APPg P TP VP.
+    specialize (PAV u v t Vu APP NB APPg P TP VP).
+    eapply Val_EqVal.
+    cbn. cbn in PAV.
+    auto.
+Defined.
 
 
 (* ValTy2-to-EqValTy2 *)
-Lemma ValTy_EqValTy {n} (Γ : Ctx n) (M : Tm n) u i (h : wt u (tuniv i)) :
+Lemma ValTy_EqValTy {n} (Γ : Ctx n) (M : Tm n) u (h : wt u tuniv) :
   ValTy Γ M h -> EqValTy Γ M M h.
 Proof.
   intros VT.
@@ -725,296 +669,93 @@ Qed.
    Head reduction/expansion
    ============================================================ *)
 
+Lemma HeadRed_expand {n} (M M' : Tm n) A B :
+  HeadRed1 M M' ->
+  HeadRed M'  (Core.tpi A B) ->
+  HeadRed M (Core.tpi A B).
+Proof.
+  move=> R HR.
+  eapply ms_trans; eauto.
+Qed.
+
+Lemma HeadRed_contract {n} (M M' : Tm n) A B :
+  HeadRed1 M M' ->
+  HeadRed M  (Core.tpi A B) ->
+  HeadRed M' (Core.tpi A B).
+Proof.
+Admitted.
+
+Lemma ValTy_HeadRed1_expand {n} (Γ : Ctx n) (M M' : Tm n) u (h : wt u tuniv) :
+  HeadRed1 M' M -> ValTy Γ M h -> ValTy Γ M' h.
+Proof. 
+  move=> R.
+  dependent destruction h.
+  all: cbn; try done.
+  move=> [A0 [B0 [R0 [TA0 [TB0 [Vpi [VA [PEV PEE]]]]]]]].
+  exists A0. exists B0.
+  repeat split; eauto.
+  eapply HeadRed_expand; eauto.
+Qed.
 
 (* ValTy2-headred-expand *)
-Lemma ValTy_headred_expand {n} (Γ : Ctx n) (M M' : Tm n) u i (h : wt u (tuniv i)) :
+Lemma ValTy_HeadRed_expand {n} (Γ : Ctx n) (M M' : Tm n) u (h : wt u tuniv) :
   HeadRed M' M -> ValTy Γ M h -> ValTy Γ M' h.
-Proof. Admitted.
-
-(* ValTy2-headred-contract *)
-Lemma ValTy_headred_contract {n} (Γ : Ctx n) (M M' : Tm n) u i (h : wt u (tuniv i)) :
-  HeadRed M M' -> ValTy Γ M h -> ValTy Γ M' h.
-Proof. Admitted.
-
-
+Proof. 
+  move=> R. induction R.
+  - done.
+  - move=> h1. specialize (IHR h1). 
+    eapply ValTy_HeadRed1_expand in H; eauto.
+Qed.
 
   
 
-(* ============================================================
-   Proof irrelevance for the mutual definitions
-   ------------------------------------------------------------
-   The tuniv case of upVal / downVal / upEqVal / downEqVal needs
-   to bridge two wt_tpi witnesses with the same indices but
-   different wt_pi_fun / wt-of-dom subderivations. ValTy at
-   wt_tpi h calls back into Val (on the dom-wt) and into
-   PiEdgeVal / PiEdgeEq (on the wt_pi_fun part), so we need
-   proof irrelevance not just for Val/EqVal but for every member
-   of the Val/EqVal/PiEdge*/PiApp* mutual block.
+Lemma ValTy_HeadRed1_contract {n} (Γ : Ctx n) (M M' : Tm n) u (h : wt u tuniv) :
+  HeadRed1 M M' -> ValTy Γ M h -> ValTy Γ M' h.
+Proof. 
+  move=> R. 
+  dependent destruction h.
+  all: cbn; try done.
+  move=> [A0 [B0 [R0 [TA0 [TB0 [Vpi [VA [PEV PEE]]]]]]]].
+  exists A0. exists B0.
+  repeat split; eauto.
+  eapply HeadRed_contract; eauto.
+Qed.
 
-   These are stated as axioms (Admitted) — they are uniform
-   "the relation does not depend on the derivation" facts about
-   each predicate in the mutual block.
+
+
+(* ValTy2-headred-contract *)
+Lemma ValTy_headred_contract {n} (Γ : Ctx n) (M M' : Tm n) u (h : wt u tuniv) :
+  HeadRed M M' -> ValTy Γ M h -> ValTy Γ M' h.
+Proof. 
+  move=> R. induction R.
+  - done.
+  - admit.
+Admitted.
+
+
+(* ============================================================
+   upValTy / downValTy — stated before the mutual block.
+
+   Each is parameterized by the mutual-block lemma its proof
+   relies on, so it can be applied inside the mutual block by
+   passing the appropriate fixpoint reference at the call site.
    ============================================================ *)
 
-Lemma ValTy_cumul {n} (Γ : Ctx n) (A : Tm n) u i (h : wt u (tuniv i)) :
-  forall j (h2 : wt u (tuniv j)), i <= j ->
-  ValTy Γ A h -> ValTy Γ A h2.
-Admitted.
-
-(* Bidirectional cross-universe ValTy proof irrelevance.
-   Required to bridge cases (wt_abs in Val/EqVal, wt_pi_cons in PiEdge)
-   where two same-shaped wt witnesses sit at unrelated universe levels;
-   the one-directional [ValTy_cumul] cannot go down. Strictly stronger
-   than [ValTy_cumul]. *)
-(*
-Lemma ValTy_pirrel_cross {n} (Γ : Ctx n) (A : Tm n) u i j
-  (h1 : wt u (tuniv i)) (h2 : wt u (tuniv j)) :
-  ValTy Γ A h1 -> ValTy Γ A h2.
-Admitted.
-
-(* Cross-universe EqValTy proof irrelevance. Same motivation as
-   [ValTy_pirrel_cross]: needed in PiEdgeEqTy / PiEdgeEq forall cases
-   where the codomain witness sits at differing universe levels. *)
-Lemma EqValTy_pirrel_cross {n} (Γ : Ctx n) (M N : Tm n) u i j
-  (h1 : wt u (tuniv i)) (h2 : wt u (tuniv j)) :
-  EqValTy Γ M N h1 -> EqValTy Γ M N h2.
-Admitted.
-*)
-
-(* The pirrel statements are proven by mutual structural induction over
-   the wt / wt_pi_fun / wt_abs_fun derivations. Cases where the inner
-   wt_abs constructor yields two different existential universes (i in
-   wt_abs's `wt (tpi a g) (tuniv i)` argument) cannot be bridged at
-   this granularity and are admitted. *)
-Fixpoint Val_pirrel {n} (Γ : Ctx n) (M A : Tm n) u a
-  (h1 h2 : wt u a) {struct h1} :
-  Val Γ M A h1 -> Val Γ M A h2
-with EqVal_pirrel {n} (Γ : Ctx n) (M N A : Tm n) u a
-  (h1 h2 : wt u a) {struct h1} :
-  EqVal Γ M N A h1 -> EqVal Γ M N A h2
-with PiEdgeVal_pirrel {n} (Γ : Ctx n)
-  (A : Tm n) (B : Tm (S n)) b f i j
-  (h1 : wt_pi_fun f b i) (h2: wt_pi_fun f b j) {struct h1} :
-  PiEdgeVal Γ A B h1 -> PiEdgeVal Γ A B h2
-with PiEdgeEq_pirrel {n} (Γ : Ctx n)
-  (A : Tm n) (B : Tm (S n)) b f i j
-  (h1 : wt_pi_fun f b i) (h2 : wt_pi_fun f b j){struct h1} :
-  PiEdgeEq Γ A B h1 -> PiEdgeEq Γ A B h2
-with PiEdgeEqTy_pirrel {n} (Γ : Ctx n)
-  (A : Tm n) (B B' : Tm (S n)) b f i j
-  (h1 : wt_pi_fun f b i) (h2 : wt_pi_fun f b j) {struct h1} :
-  PiEdgeEqTy Γ A B B' h1 -> PiEdgeEqTy Γ A B B' h2
-with PiAppVal_pirrel {n} (Γ : Ctx n)
-  (M : Tm n) (A0 : Tm n) (B0 : Tm (S n)) f b g
-  (h1 h2 : wt_abs_fun f b g) {struct h1} :
-  PiAppVal Γ M A0 B0 h1 -> PiAppVal Γ M A0 B0 h2
-with PiAppEq_pirrel {n} (Γ : Ctx n)
-  (M : Tm n) (A0 : Tm n) (B0 : Tm (S n)) f b g
-  (h1 h2 : wt_abs_fun f b g) {struct h1} :
-  PiAppEq Γ M A0 B0 h1 -> PiAppEq Γ M A0 B0 h2
-with PiAppEqVal_pirrel {n} (Γ : Ctx n)
-  (M N : Tm n) (A0 : Tm n) (B0 : Tm (S n)) f b g
-  (h1 h2 : wt_abs_fun f b g) {struct h1} :
-  PiAppEqVal Γ M N A0 B0 h1 -> PiAppEqVal Γ M N A0 B0 h2
-
-with ValTy_pirrel_cross {n} (Γ : Ctx n) (A : Tm n) u i j
-  (h1 : wt u (tuniv i)) (h2 : wt u (tuniv j)) :
-  ValTy Γ A h1 -> ValTy Γ A h2
-with EqValTy_pirrel_cross {n} (Γ : Ctx n) (M N : Tm n) u i j
-  (h1 : wt u (tuniv i)) (h2 : wt u (tuniv j)) :
-  EqValTy Γ M N h1 -> EqValTy Γ M N h2.
+(* downValTy: shrink the term-side element u (same type tuniv).
+   Derivable from [restrictVal] of the mutual block. *)
+Lemma downValTy_pre
+  (restrictVal :
+    forall n (Γ : Ctx n) (M T : Tm n) u u' a
+           (h0 : wt u' a) (h1 : wt u a),
+           le u' u -> Val Γ M T h1 -> Val Γ M T h0)
+  {n} (Γ : Ctx n) (M : Tm n) u0 u1
+  (h0 : wt u0 tuniv) (h1 : wt u1 tuniv) :
+  le u0 u1 -> ValTy Γ M h1 -> ValTy Γ M h0.
 Proof.
-  - (* Val_pirrel *)
-    intros VAL.
-    have 
-      ValTy_pirrel : forall n (Γ : Ctx n) (A : Tm n) u i 
-        (h1 : wt u (tuniv i)) j (h2 : wt u (tuniv j)),
-        ValTy Γ A h1 -> ValTy Γ A h2.
-    { 
-      clear n Γ M A u a h1 h2 VAL.
-      move=> n Γ A u i h1 j h2 VT.
-      dependent destruction h1; dependent destruction h2.
-      all: try solve [cbn; done].
-      cbn in VT |- *.
-      destruct VT as (A0 & B0 & R1 (* & T1 & T2 *) & VV & Vh1 & PEV & PEE).
-      exists A0. exists B0. 
-      split. exact R1.
-(*      split. exact T1.
-      split. exact T2. *)       
-      admit.
-(*      split. exact VV.
-      split. eapply Val_pirrel; eauto.
-      split. eapply PiEdgeVal_pirrel; eauto.
-      eapply PiEdgeEq_pirrel; eauto. *)
-    }
-    dependent destruction h1; dependent destruction h2.
-    + (* wt_bot *) destruct a; cbn in *; trivial.
-    + (* wt_tuniv *) cbn in *; trivial.
-    + (* wt_tnat *) cbn in *; trivial.
-    + (* wt_zero *) cbn in *; exact VAL.
-    + (* wt_succ *)
-      cbn in *.
-      destruct VAL as [M1 [HR VM1]].
-      exists M1. split; [exact HR | eapply Val_pirrel; exact VM1].
-    + (* wt_tpi *)
-      cbn in *.
-      destruct VAL as (A0 & B0 & HR (* & TA & TB *) & V & VD & PEV & PEE).
-      exists A0, B0. split; [exact HR|].
-      (* split; [exact TA|]. split; [exact TB|].  *)
-         split; [exact V|].
-      split; [eapply Val_pirrel; exact VD|].
-      split; [eapply PiEdgeVal_pirrel; exact PEV
-             |eapply PiEdgeEq_pirrel; exact PEE].
-    + (* wt_abs: destruct inner wt_tpi to expose universes, bridge with cross-PI *)
-      match goal with H : wt (tpi _ _) (tuniv _) |- _ => dependent destruction H end.
-      match goal with H : wt (tpi _ _) (tuniv _) |- _ => dependent destruction H end.
-      cbn in VAL |- *.
-      destruct VAL as [VT VP].
-      split.
-      * eapply ValTy_pirrel_cross. exact VT.
-      * destruct VP as (A0 & B0 & HR & PA).
-        exists A0, B0. split; [exact HR|].
-        eapply PiAppVal_pirrel. exact PA.
-  - (* EqVal_pirrel *)
-    intros EV.
-    dependent destruction h1; dependent destruction h2.
-    + (* wt_bot *) destruct a; cbn in *; trivial.
-    + (* wt_tuniv *) cbn in *; exact EV.
-    + (* wt_tnat *) cbn in *; trivial.
-    + (* wt_zero *) cbn in *; exact EV.
-    + (* wt_succ *)
-      cbn in *.
-      destruct EV as [M1 [HR1 [N1 [HR2 EV']]]].
-      exists M1. split; [exact HR1|].
-      exists N1. split; [exact HR2|].
-      eapply EqVal_pirrel; exact EV'.
-    + (* wt_tpi: same i, bridge ValTy x2 + EqValTy components *)
-      cbn in EV |- *.
-      fold (valid_fun g) in EV.
-      destruct EV as [VTm [VTn EVT]].
-      admit.
-     
-
-(*    split.  move: (ValTy_pirrel_cross Γ M w j 
-      split; [eapply ValTy_pirrel_cross; exact VTm|].
-      split; [eapply ValTy_pirrel_cross; exact VTn|].
-      destruct EVT as (VTm' & VTn' & A0 & B0 & HRm & A0' & B0' & HRn
-                       & TC1 & TC2 & VPI & EVD & PEET).
-      split; [eapply ValTy_pirrel_cross; exact VTm'|].
-      split; [eapply ValTy_pirrel_cross; exact VTn'|].
-      exists A0, B0. split; [exact HRm|].
-      exists A0', B0'. split; [exact HRn|].
-      split; [exact TC1|]. split; [exact TC2|]. split; [exact VPI|].
-      split.
-      * eapply EqVal_pirrel; exact EVD.
-      * eapply PiEdgeEqTy_pirrel; exact PEET. *)
-    + (* wt_abs: bridge inner wt_tpi via cross-PI; recurse on ValPi/EqValPi parts *)
-      match goal with H : wt (tpi _ _) (tuniv _) |- _ => dependent destruction H end.
-      match goal with H : wt (tpi _ _) (tuniv _) |- _ => dependent destruction H end.
-      cbn in EV |- *.
-      destruct EV as [VT [VPm [VPn EVPm]]].
-      destruct VPm as (A0 & B0 & HRm & PAm).
-      destruct VPn as (A0' & B0' & HRn & PAn).
-      destruct EVPm as (A0'' & B0'' & HRe & EPA).
-      split; [eapply ValTy_pirrel_cross; exact VT|].
-      split.
-      { exists A0, B0. split; [exact HRm|]. eapply PiAppVal_pirrel; exact PAm. }
-      split.
-      { exists A0', B0'. split; [exact HRn|]. eapply PiAppVal_pirrel; exact PAn. }
-      exists A0'', B0''. split; [exact HRe|]. eapply PiAppEqVal_pirrel; exact EPA.
-  - (* PiEdgeVal_pirrel *)
-    intros PE.
-    dependent destruction h1; dependent destruction h2.
-    + (* wt_pi_nil *) cbn. trivial.
-    + (* wt_pi_cons *)
-      cbn in PE. destruct PE as [PE_rec PE_forall].
-      cbn. split.
-      * eapply PiEdgeVal_pirrel; exact PE_rec.
-      * intros N TN VN.
-        (* Goal at cross-universe j; bridge via ValTy_pirrel_cross *)
-        apply ValTy_Val.
-        eapply ValTy_pirrel_cross.
-        apply Val_ValTy.
-        apply (PE_forall N TN).
-        eapply Val_pirrel. exact VN.
-  - (* PiEdgeEq_pirrel *)
-    intros PE.
-    dependent destruction h1; dependent destruction h2.
-    + cbn. trivial.
-    + cbn in PE. destruct PE as [PE_rec PE_forall].
-      cbn. split.
-      * eapply PiEdgeEq_pirrel; exact PE_rec.
-      * intros N1 N2 CV EV.
-        apply EqValTy_EqVal.
-        eapply EqValTy_pirrel_cross.
-        eapply EqVal_EqValTy.
-        apply (PE_forall N1 N2 CV).
-        eapply EqVal_pirrel. exact EV.
-  - (* PiEdgeEqTy_pirrel *)
-    intros PE.
-    dependent destruction h1; dependent destruction h2.
-    + cbn. trivial.
-    + cbn in PE. destruct PE as [PE_rec PE_forall].
-      cbn. split.
-      * eapply PiEdgeEqTy_pirrel; exact PE_rec.
-      * intros P TP VP.
-        eapply EqValTy_pirrel_cross.
-        apply (PE_forall P TP).
-        eapply Val_pirrel. exact VP.
-  - (* PiAppVal_pirrel *)
-    intros PA.
-    dependent destruction h1; dependent destruction h2.
-    + cbn. trivial.
-    + cbn in PA. destruct PA as [PA_rec PA_forall].
-      cbn. split.
-      * eapply PiAppVal_pirrel; exact PA_rec.
-      * intros P TP VP.
-        (* Equate the two app g ui = Some _ witnesses to align cod-types. *)
-        match goal with
-        | E1 : app ?g0 ?u0 = Some ?t1,
-          E2 : app ?g0 ?u0 = Some ?t2 |- _ => 
-            assert (Heq : t1 = t2) by congruence;         
-            try subst t1; try subst t2
-        end.
-        eapply Val_pirrel.
-        apply (PA_forall P TP).
-        eapply Val_pirrel. exact VP.
-  - (* PiAppEq_pirrel *)
-    intros PA.
-    dependent destruction h1; dependent destruction h2.
-    + cbn. trivial.
-    + cbn in PA. destruct PA as [PA_rec PA_forall].
-      cbn. split.
-      * eapply PiAppEq_pirrel; exact PA_rec.
-      * intros N1 N2 CV EV.
-        match goal with
-        | E1 : app ?g0 ?u0 = Some ?t1,
-          E2 : app ?g0 ?u0 = Some ?t2 |- _ =>
-            assert (Heq : t1 = t2) by congruence;
-            try subst t1; try subst t2 (* ; clear Heq *)
-        end.
-        eapply EqVal_pirrel.
-        apply (PA_forall N1 N2 CV).
-        eapply EqVal_pirrel. exact EV.
-  - (* PiAppEqVal_pirrel *)
-    intros PA.
-    dependent destruction h1; dependent destruction h2.
-    + cbn. trivial.
-    + cbn in PA. destruct PA as [PA_rec PA_forall].
-      cbn. split.
-      * eapply PiAppEqVal_pirrel; exact PA_rec.
-      * intros P TP VP.
-        match goal with
-        | E1 : app ?g0 ?u0 = Some ?t1,
-          E2 : app ?g0 ?u0 = Some ?t2 |- _ =>
-            assert (Heq : t1 = t2) by congruence;
-            try subst t1; try subst t2 (* ; clear Heq *)
-        end.
-        eapply EqVal_pirrel.
-        apply (PA_forall P TP).
-        eapply Val_pirrel. exact VP.
-Admitted.
-(* Qed. *)
+  move=> LE VT1.
+  apply Val_ValTy. apply ValTy_Val in VT1.
+  eapply restrictVal; eauto.
+Qed.
 
 
 (* ============================================================
@@ -1030,29 +771,30 @@ Admitted.
 
 (* upVal/upEqVal mirror the Agda upVal2/upEqVal2 signatures: they take
    the ValTy of the syntactic type T at the bigger universe-element a1
-   as an extra argument (a "Val Γ T (Core.tuniv i) hUa1", which by
+   as an extra argument (a "Val Γ T Core.tuniv hUa1", which by
    definitional unfolding is ValTy Γ T hUa1).                          *)
 Fixpoint upVal {n} (Γ : Ctx n) (M T : Tm n) u a0 a1
-  (h0 : wt u a0) (h1 : wt u a1) i 
-  (hUa0 : wt a0 (tuniv i)) (hUa1 : wt a1 (tuniv i)) {struct h1}:
-  le a0 a1 -> Val Γ M T h0 -> Val Γ T (Core.tuniv i) hUa1 -> Val Γ M T h1
+  (h0 : wt u a0) (h1 : wt u a1)  
+  (hUa0 : wt a0 tuniv) (hUa1 : wt a1 tuniv) {struct h1}:
+  le a0 a1 -> Val Γ M T h0 -> Val Γ T Core.tuniv hUa1 -> Val Γ M T h1
 with upEqVal {n} (Γ : Ctx n) (M N T : Tm n) u a0 a1
-  (h0 : wt u a0) (h1 : wt u a1) i 
-  (hUa0 : wt a0 (tuniv i)) (hUa1 : wt a1 (tuniv i)) {struct h1}:
-  le a0 a1 -> EqVal Γ M N T h0 -> Val Γ T (Core.tuniv i) hUa1 -> EqVal Γ M N T h1
+  (h0 : wt u a0) (h1 : wt u a1)  
+  (hUa0 : wt a0 tuniv) (hUa1 : wt a1 tuniv) {struct h1}:
+  le a0 a1 -> EqVal Γ M N T h0 -> Val Γ T Core.tuniv hUa1 -> EqVal Γ M N T h1
 with downVal {n} (Γ : Ctx n) (M T : Tm n) u a0 a1
   (h0 : wt u a0) (h1: wt u a1) {struct h1} :
   le a0 a1 -> Val Γ M T h1 -> Val Γ M T h0
 with downEqVal {n} (Γ : Ctx n) (M N T : Tm n) u a0 a1
   (h0 : wt u a0) (h1: wt u a1) {struct h1} :
   le a0 a1 -> EqVal Γ M N T h1 -> EqVal Γ M N T h0
+(*
 (* -------- Pi helper lemmas (mutual with Val/EqVal) --------
    The up* helpers mirror Agda's upPiAppVal2 / upPiAppEq2 / upPiAppEqVal2
    by additionally taking PiEdgeVal at the bigger pi (hPi1) — this
    supplies the ValTy of the codomain at the bigger universe-element,
    needed to invoke upVal/upEqVal on the codomain.                    *)
 with upPiAppVal {n} (Γ : Ctx n) (M : Tm n) (A0 : Tm n) (B0 : Tm (S n))
-  f b0 b1 g0 g1 i (hPi : wt_pi_fun g0 b0 i) (hPi1 : wt_pi_fun g1 b1 i)
+  f b0 b1 g0 g1 (hPi0 : wt_pi_fun g0 b0) (hPi1 : wt_pi_fun g1 b1)
   (h0 : wt_abs_fun f b0 g0) (h1 : wt_abs_fun f b1 g1) {struct h0} :
   le b0 b1 -> le_fun g0 g1 ->
   PiEdgeVal Γ A0 B0 hPi1 ->
@@ -1063,7 +805,7 @@ with downPiAppVal {n} (Γ : Ctx n) (M : Tm n) (A0 : Tm n) (B0 : Tm (S n))
   le b0 b1 -> le_fun g0 g1 ->
   PiAppVal Γ M A0 B0 h1 -> PiAppVal Γ M A0 B0 h0
 with upPiAppEq {n} (Γ : Ctx n) (M : Tm n) (A0 : Tm n) (B0 : Tm (S n))
-  f b0 b1 g0 g1 i (hPi0 : wt_pi_fun g0 b0 i) (hPi1 : wt_pi_fun g1 b1 i)
+  f b0 b1 g0 g1 (hPi0 : wt_pi_fun g0 b0) (hPi1 : wt_pi_fun g1 b1)
   (h0 : wt_abs_fun f b0 g0) (h1 : wt_abs_fun f b1 g1) {struct h0} :
   le b0 b1 -> le_fun g0 g1 ->
   PiEdgeVal Γ A0 B0 hPi1 ->
@@ -1074,7 +816,7 @@ with downPiAppEq {n} (Γ : Ctx n) (M : Tm n) (A0 : Tm n) (B0 : Tm (S n))
   le b0 b1 -> le_fun g0 g1 ->
   PiAppEq Γ M A0 B0 h1 -> PiAppEq Γ M A0 B0 h0
 with upPiAppEqVal {n} (Γ : Ctx n) (M N : Tm n) (A0 : Tm n) (B0 : Tm (S n))
-  f b0 b1 g0 g1 i (hPi0 : wt_pi_fun g0 b0 i) (hPi1 : wt_pi_fun g1 b1 i)
+  f b0 b1 g0 g1 (hPi0 : wt_pi_fun g0 b0) (hPi1 : wt_pi_fun g1 b1)
   (h0 : wt_abs_fun f b0 g0) (h1 : wt_abs_fun f b1 g1) {struct h0} :
   le b0 b1 -> le_fun g0 g1 ->
   PiEdgeVal Γ A0 B0 hPi1 ->
@@ -1085,21 +827,29 @@ with downPiAppEqVal {n} (Γ : Ctx n) (M N : Tm n) (A0 : Tm n) (B0 : Tm (S n))
   le b0 b1 -> le_fun g0 g1 ->
   PiAppEqVal Γ M N A0 B0 h1 -> PiAppEqVal Γ M N A0 B0 h0
 with downPiEdgeVal {n} (Γ : Ctx n) (A : Tm n) (B : Tm (S n))
-  b0 b1 f0 f1 i
-  (h0 : wt_pi_fun f0 b0 i) (h1 : wt_pi_fun f1 b1 i) {struct h0} :
+  b0 b1 f0 f1 
+  (h0 : wt_pi_fun f0 b0 ) (h1 : wt_pi_fun f1 b1 ) {struct h0} :
   le b0 b1 -> le_fun f0 f1 ->
   PiEdgeVal Γ A B h1 -> PiEdgeVal Γ A B h0
 with downPiEdgeEq {n} (Γ : Ctx n) (A : Tm n) (B : Tm (S n))
-  b0 b1 f0 f1 i
-  (h0 : wt_pi_fun f0 b0 i) (h1 : wt_pi_fun f1 b1 i) {struct h0} :
+  b0 b1 f0 f1 
+  (h0 : wt_pi_fun f0 b0 ) (h1 : wt_pi_fun f1 b1 ) {struct h0} :
   le b0 b1 -> le_fun f0 f1 ->
   PiEdgeEq Γ A B h1 -> PiEdgeEq Γ A B h0
 with downPiEdgeEqTy {n} (Γ : Ctx n) (A : Tm n) (B B' : Tm (S n))
-  b0 b1 f0 f1 i
-  (h0 : wt_pi_fun f0 b0 i) (h1 : wt_pi_fun f1 b1 i) {struct h0} :
+  b0 b1 f0 f1
+  (h0 : wt_pi_fun f0 b0 ) (h1 : wt_pi_fun f1 b1 ) {struct h0} :
   le b0 b1 -> le_fun f0 f1 ->
-  PiEdgeEqTy Γ A B B' h1 -> PiEdgeEqTy Γ A B B' h0.
-Proof.
+  PiEdgeEqTy Γ A B B' h1 -> PiEdgeEqTy Γ A B B' h0
+*)
+(* -------- restrictVal / restrictEqVal (moved into the mutual block) -------- *)
+with restrictVal {n} (Γ : Ctx n) (M T : Tm n) u u' a
+  (h0 : wt u' a) (h1 : wt u a) {struct h1} :
+  le u' u -> Val Γ M T h1 -> Val Γ M T h0
+with restrictEqVal {n} (Γ : Ctx n) (M N T : Tm n) u u' a
+  (h0 : wt u' a) (h1 : wt u a) {struct h1} :
+  le u' u -> EqVal Γ M N T h1 -> EqVal Γ M N T h0.
+Proof.  
   - (* upVal *)
     dependent destruction h1;
     dependent destruction h0.
@@ -1110,23 +860,31 @@ Proof.
       move=> _ h3 _. cbn in h3. move: h3 => [M1 [RM1 VM1]].
       exists M1. split. auto. 
       cbn.
-      eapply Val_pirrel; eauto.
+      rewrite (wt_unique h0 h1) in VM1.
+      done.
 
-    + (* tuniv *)
+    + (* tuniv: explicit ValTy destructure + rewrites identify the inner
+         witnesses (mirrors the working upVal tuniv proof shape). *)
       move=> LE VT _.
-      cbn in LE.
-      apply Nat.eqb_eq in LE. subst j0.
-      (* h0 and h1 are two wt_tpi derivations of (tpi a g) at (tuniv j).
-         Val at either reduces to ValTy, whose substructure (Val on the
-         dom-wt, PiEdgeVal/PiEdgeEq on the wt_pi_fun) differs only in the
-         derivation choice. Bridge with the Val proof-irrelevance axiom. *)
-      eapply Val_pirrel; exact VT.
+      cbn in VT |- *.
+      destruct VT as (A0 & B0 & RA & TA0 & TB0 & VTpi & VV & PEV & PEE).
+(*      rewrite (wt_pi_fun_unique w w0) in PEV, PEE. *)
+      rewrite (wt_unique h0 h1) in VV.
+      exists A0, B0; repeat split; try eassumption.
+      move=> u v Vu APP NB WTu N TN VN.
+      specialize (PEV u v Vu APP NB WTu N TN).
+      rewrite (wt_unique (w1 u v Vu APP NB) (w u v Vu APP NB)) in VN.
+      specialize (PEV VN).
+      erewrite (wt_unique (w0 u v Vu APP NB)) in PEV. eapply PEV.
+      unfold Rec.PiEdgeEq.
+      move=> u v Vu APP NB WTu N TN VN.
+      specialize (PEE u v Vu APP NB WTu N TN).
+      cbn in PEE. cbn in VN.
+      rewrite (wt_unique (w1 u v Vu APP NB) (w u v Vu APP NB)) in VN.
+      specialize (PEE VN).
+      cbn.
+      erewrite (wt_unique (w0 u v Vu APP NB)) in PEE. eapply PEE.
     + (* tpi *)
-      (* Mirror Agda Validity2.agda: upVal2 PiCode case.
-         Use the new ValTy arg (Val Γ T (Core.tuniv i) hUa1) to supply
-         the first conjunct of Val at h1 (ValTy at the bigger dom).
-         Use upPiAppVal — passing PiEdgeVal extracted from the ValTy arg —
-         for the ValPi part. *)
       dependent destruction h0.
       dependent destruction h1.
       rewrite le_tpi.
@@ -1134,20 +892,26 @@ Proof.
       apply andb_prop in LE.
       destruct LE as [LEa LEg].
       move=> VAL VTa1.
-      cbn in VAL. 
-      unfold Rec.ValPi in VAL.
+      cbn in VAL. fold ValTy in VAL. 
       destruct VAL as [VT VP].
+      unfold Rec.ValPi in VP. 
       destruct VP as [A0 [B0 [R1 PAV]]].
       cbn. split.
-      * (* ValTy at WTb_h1 (the bigger pi's dom witness).
-           The new ValTy arg VTa1 is at the WHOLE bigger pi (hUa1 : wt a1 (tuniv i)),
-           not at the dom — they're structurally different. Bridging requires
-           extracting the dom-Val from the pi-ValTy existentials + universe-aware
-           proof irrelevance. Admit this bridging step. *)
-        admit.
-      * unfold Rec.ValPi. exists A0, B0. split. exact R1.
-        (* Apply upPiAppVal with the new PiEdgeVal arg (extracted from VTa1) *)
-        admit.
+      * eapply Val_ValTy in VTa1.
+(* TODO: update proofs from here *)
+
+        destruct VTa1 as (Av & Bv & HRv & TAv & TBv & VPi & VDv & PEVv & PEEv).
+        exists Av. exists Bv.
+        rewrite (wt_unique (wt_tpi_dom hUa1) h1) in VDv. 
+        rewrite (wt_pi_fun_unique (wt_tpi_inv hUa1) w2) in PEVv, PEEv.
+        repeat split; eauto.
+      * unfold Rec.ValPi. exists A0, B0. split; [exact R1|].
+        apply Val_ValTy in VTa1.
+        cbn in VTa1.
+        destruct VTa1 as (Av & Bv & HRv & TAv & TBv & VPi & VDv & PEVv & PEEv).
+        destruct (HeadRed_tpi_det HRv R1) as [EqA EqB]. subst.
+        rewrite (wt_pi_fun_unique (wt_tpi_inv hUa1) w2) in PEVv.
+        exact (@upPiAppVal _ _ _ _ _ _ _ _ _ _ w0 w2 w w1 LEa LEg PEVv PAV).
   - (* upEqVal *)
     dependent destruction h1;
     dependent destruction h0.
@@ -1155,16 +919,46 @@ Proof.
     + (* bot *)
       destruct a; destruct a0; cbn; auto.
     + (* tnat *)
-      move=> _ [M1 [RM1 [N1 [RN1 VM1]]]] _.
+      move=> _ [M1 [RM1 [N1 [RN1 EVM]]]] _.
       exists M1. split. auto.
       exists N1. split. auto.
-      eapply upEqVal with (a1 := tnat) (i := 0) (hUa1 := wt_tnat 0); admit.
-    + (* tuniv *)
-      (* Bridge two wt_tpi witnesses at same indices via EqVal_pirrel. *)
+      rewrite (wt_unique h0 h1) in EVM.
+      done.
+    + (* tuniv: split EqVal at tuniv into ValTy/ValTy/EqValTy, then rewrite
+         each component to point at h1's destructured inner witnesses. *)
       move=> LE EV _.
-      cbn in LE.
-      apply Nat.eqb_eq in LE. subst j0.
-      eapply EqVal_pirrel; exact EV.
+      cbn in EV |- *.
+      destruct EV as [VTm [VTn EVT]].
+      split; [|split].
+      * (* ValTy Γ M h1 *)
+        destruct VTm as (Am & Bm & RAm & TAm & TBm & Vpim & VVm & PEVm & PEEm).
+        rewrite (wt_pi_fun_unique w w0) in PEVm, PEEm.
+        rewrite (wt_unique h0 h1) in VVm.
+        exists Am, Bm; repeat split; eassumption.
+      * (* ValTy Γ N h1 *)
+        destruct VTn as (An & Bn & RAn & TAn & TBn & Vpin & VVn & PEVn & PEEn).
+        rewrite (wt_pi_fun_unique w w0) in PEVn, PEEn.
+        rewrite (wt_unique h0 h1) in VVn.
+        exists An, Bn; repeat split; eassumption.
+      * (* EqValTy Γ M N h1 *)
+        cbn in EVT |- *.
+        destruct EVT as (VTmE & VTnE & Ae & Be & RAe & Ae' & Be' & RAe' &
+                         CA & CB & VTpie & EVD & PEET).
+        split.
+        { destruct VTmE as (AmE & BmE & RAmE & TAmE & TBmE & VpimE & VVmE & PEVmE & PEEmE).
+          rewrite (wt_pi_fun_unique w w0) in PEVmE, PEEmE.
+          rewrite (wt_unique h0 h1) in VVmE.
+          exists AmE, BmE; repeat split; eassumption. }
+        split.
+        { destruct VTnE as (AnE & BnE & RAnE & TAnE & TBnE & VpinE & VVnE & PEVnE & PEEnE).
+          rewrite (wt_pi_fun_unique w w0) in PEVnE, PEEnE.
+          rewrite (wt_unique h0 h1) in VVnE.
+          exists AnE, BnE; repeat split; eassumption. }
+        exists Ae, Be; split; [exact RAe|].
+        exists Ae', Be'; split; [exact RAe'|].
+        rewrite (wt_pi_fun_unique w w0) in PEET.
+        rewrite (wt_unique h0 h1) in EVD.
+        repeat split; eassumption.
     + (* tpi *)
       (* Mirror Agda Validity2.agda: upEqVal2 PiCode case.
          EqVal at (abs f) (tpi a g) is ValTy /\ ValPi M /\ ValPi N /\ EqValPi M N.
@@ -1183,11 +977,28 @@ Proof.
       destruct VPM as [A0_M [B0_M [R_M PAV_M]]].
       destruct VPN as [A0_N [B0_N [R_N PAV_N]]].
       destruct EPI as [A0_E [B0_E [R_E PAEV]]].
+      apply Val_ValTy in VTa1.
+      cbn in VTa1.
+      destruct VTa1 as (Av & Bv & HRv & TAv & TBv & VPi & VDv & PEVv & PEEv).
       cbn. split; [|split; [|split]].
-      * admit. (* ValTy bridging *)
-      * unfold Rec.ValPi. exists A0_M, B0_M. split. exact R_M. admit.
-      * unfold Rec.ValPi. exists A0_N, B0_N. split. exact R_N. admit.
-      * unfold Rec.EqValPi. exists A0_E, B0_E. split. exact R_E. admit.
+      * exists A0_M, B0_M.        
+        destruct (HeadRed_tpi_det HRv R_M) as [EqA EqB]. subst.
+        rewrite (wt_pi_fun_unique (wt_tpi_inv hUa1) w2) in PEVv, PEEv.
+        rewrite (wt_unique (wt_tpi_dom hUa1) h1) in VDv.
+        repeat split; eauto.
+
+      * unfold Rec.ValPi. exists A0_M, B0_M. split; [exact R_M|].
+        destruct (HeadRed_tpi_det HRv R_M) as [EqA EqB]. subst.
+        rewrite (wt_pi_fun_unique (wt_tpi_inv hUa1) w2) in PEVv.
+        exact (@upPiAppVal _ _ _ _ _ _ _ _ _ _ w0 w2 w w1 LEa LEg PEVv PAV_M).
+      * unfold Rec.ValPi. exists A0_N, B0_N. split; [exact R_N|].
+        destruct (HeadRed_tpi_det HRv R_N) as [EqA EqB]. subst.
+        rewrite (wt_pi_fun_unique (wt_tpi_inv hUa1) w2) in PEVv.
+        exact (@upPiAppVal _ _ _ _ _ _ _ _ _ _ w0 w2 w w1 LEa LEg PEVv PAV_N).
+      * unfold Rec.EqValPi. exists A0_E, B0_E. split; [exact R_E|].
+        destruct (HeadRed_tpi_det HRv R_E) as [EqA EqB]. subst.
+        rewrite (wt_pi_fun_unique (wt_tpi_inv hUa1) w2) in PEVv.
+        exact (@upPiAppEqVal _ _ _ _ _ _ _ _ _ _ _ w0 w2 w w1 LEa LEg PEVv PAEV).
 
   - (* downVal *)
     dependent destruction h1;
@@ -1196,20 +1007,19 @@ Proof.
     + (* bot *)
       destruct a; destruct a0; cbn; auto; done.
     + (* tnat *)
-      all: move=> _ [M1 [RM1 VM1]].
-       exists M1. split. auto.
-      eapply downVal with (a1 := tnat); eauto. 
-    + (* tuniv *)
-      (* Bridge two wt_tpi witnesses at same indices via Val_pirrel. *)
+      move=> _ [M1 [RM1 VM1]].
+      exists M1. split. auto.
+      rewrite (wt_unique h1 h0) in VM1.
+      done.
+    + (* tuniv: same pattern as upVal, but going h1 → h0. *)
       move=> LE VT.
-      cbn in LE.
-      apply Nat.eqb_eq in LE. subst j0.
-      eapply Val_pirrel; exact VT.
+      cbn in VT |- *.
+      destruct VT as (A0 & B0 & RA & TA0 & TB0 & VTpi & VV & PEV & PEE).
+      rewrite (wt_pi_fun_unique w0 w) in PEV, PEE.
+      rewrite (wt_unique h1 h0) in VV.
+      exists A0, B0; repeat split; eassumption.
     + (* tpi *)
-      (* Mirror Agda Validity2.agda: downVal2 PiCode case.
-         Convert Val at h1 (bigger pi a0/g0) to Val at h0 (smaller pi a/g):
-           - downValTy on the domain ValTy   (admit: universe alignment)
-           - downPiAppVal on the PiAppVal    (mutual)                       *)
+      have Vag: valid (tpi a g).  eauto with valid.
       dependent destruction h0.
       dependent destruction h1.
       rewrite le_tpi.
@@ -1217,40 +1027,63 @@ Proof.
       apply andb_prop in LE.
       destruct LE as [LEa LEg].
       move=> VAL.
-      cbn in VAL.
-      unfold Rec.ValPi in VAL.
-      destruct VAL as [VT VP].
-      destruct VP as [A0 [B0 [R1 PAV]]].
-      cbn. split.
-      * (* ValTy at smaller WTb_h0 from ValTy at WTb_h1.
-           Mirrors Agda's `downValTy2 _ _ (PiCode b0 f0) (PiCode b1 f1) ...`.
-           The Rocq `downValTy` requires identical universe indices on
-           both wt witnesses; here `i` and `i1` are taken from h0/h1's
-           wt_tpi destructions and are not syntactically equal, so this
-           step also needs universe alignment (proof irrelevance for the
-           universe index, beyond the same-index `Val_pirrel`). *)
-        admit.
-      * unfold Rec.ValPi. exists A0, B0. split. exact R1.
+      cbn in VAL. fold ValTy in VAL. destruct VAL as [VT VP].
+      cbn. fold ValPi. split.
+      * destruct VT as (Am & Bm & RAm & TAm & TBm & Vpim & VVm & PEVm & PEEm).
+        exists Am, Bm.
+        repeat split; try eassumption.
+        eapply restrictVal; eauto.
+        eapply downPiEdgeVal; eauto.
+        eapply downPiEdgeEq; eauto.
+      * destruct VP as [A0 [B0 [R1 PAV]]].
+        unfold Rec.ValPi. exists A0, B0. split. exact R1.
         eapply downPiAppVal; eauto.
   - (* downEqVal *)
     dependent destruction h1;
     dependent destruction h0.
     all: try solve [cbn; eauto].
     + destruct a; destruct a0; cbn; auto; done.
-    + move=> _ [M1 [RM1 [N1 [RN1 VM1]]]].
+    + move=> _ [M1 [RM1 [N1 [RN1 EVM]]]].
       exists M1. split. auto.
       exists N1. split. auto.
-      eapply downEqVal with (a1 := tnat); eauto.
-    + (* tuniv *)
-      (* Bridge two wt_tpi witnesses at same indices via EqVal_pirrel. *)
+      rewrite (wt_unique h1 h0) in EVM.
+      done.
+    + (* tuniv: split EqVal then rewrite each component (going h1 → h0). *)
       move=> LE EV.
-      cbn in LE.
-      apply Nat.eqb_eq in LE. subst j0.
-      eapply EqVal_pirrel; exact EV.
+      cbn in EV |- *.
+      destruct EV as [VTm [VTn EVT]].
+      split; [|split].
+      * destruct VTm as (Am & Bm & RAm & TAm & TBm & Vpim & VVm & PEVm & PEEm).
+        rewrite (wt_pi_fun_unique w0 w) in PEVm, PEEm.
+        rewrite (wt_unique h1 h0) in VVm.
+        exists Am, Bm; repeat split; eassumption.
+      * destruct VTn as (An & Bn & RAn & TAn & TBn & Vpin & VVn & PEVn & PEEn).
+        rewrite (wt_pi_fun_unique w0 w) in PEVn, PEEn.
+        rewrite (wt_unique h1 h0) in VVn.
+        exists An, Bn; repeat split; eassumption.
+      * cbn in EVT |- *.
+        destruct EVT as (VTmE & VTnE & Ae & Be & RAe & Ae' & Be' & RAe' &
+                         CA & CB & VTpie & EVD & PEET).
+        split.
+        { destruct VTmE as (AmE & BmE & RAmE & TAmE & TBmE & VpimE & VVmE & PEVmE & PEEmE).
+          rewrite (wt_pi_fun_unique w0 w) in PEVmE, PEEmE.
+          rewrite (wt_unique h1 h0) in VVmE.
+          exists AmE, BmE; repeat split; eassumption. }
+        split.
+        { destruct VTnE as (AnE & BnE & RAnE & TAnE & TBnE & VpinE & VVnE & PEVnE & PEEnE).
+          rewrite (wt_pi_fun_unique w0 w) in PEVnE, PEEnE.
+          rewrite (wt_unique h1 h0) in VVnE.
+          exists AnE, BnE; repeat split; eassumption. }
+        exists Ae, Be; split; [exact RAe|].
+        exists Ae', Be'; split; [exact RAe'|].
+        rewrite (wt_pi_fun_unique w0 w) in PEET.
+        rewrite (wt_unique h1 h0) in EVD.
+        repeat split; eassumption.
     + (* tpi *)
       (* Mirror Agda Validity2.agda: downEqVal2 PiCode case.
          EqVal at (abs f) (tpi a g) is
             ValTy /\ ValPi M /\ ValPi N /\ EqValPi M N. *)
+      have Vtpi : valid (tpi a g). eauto with valid.
       dependent destruction h0.
       dependent destruction h1.
       rewrite le_tpi.
@@ -1265,47 +1098,111 @@ Proof.
       destruct VPN as [A0_N [B0_N [R_N PAV_N]]].
       destruct EPI as [A0_E [B0_E [R_E PAEV]]].
       cbn. split; [|split; [|split]].
-      * (* ValTy at smaller (proof irrelevance / universe alignment) *)
-        admit.
+      * destruct VT as (Am & Bm & RAm & TAm & TBm & Vpim & VVm & PEVm & PEEm).
+        exists Am, Bm.
+        repeat split; try eassumption.
+        eapply restrictVal; eauto.
+        eapply downPiEdgeVal; eauto.
+        eapply downPiEdgeEq; eauto.
       * unfold Rec.ValPi. exists A0_M, B0_M. split. exact R_M.
         eapply downPiAppVal; eauto.
       * unfold Rec.ValPi. exists A0_N, B0_N. split. exact R_N.
         eapply downPiAppVal; eauto.
       * unfold Rec.EqValPi. exists A0_E, B0_E. split. exact R_E.
         eapply downPiAppEqVal; eauto.
-  - (* upPiAppVal: takes extra PiEdgeVal at the bigger pi (mirror of Agda's piEV1) *)
-    intros LE LEg PEV PA.
+  - (* upPiAppVal: takes extra PiEdgeVal 
+       at the bigger pi (mirror of Agda's piEV1). *)
+    intros LE LEg piEV1 PA.
     dependent destruction h0.
-    + (* wt_abs_nil: PiAppVal at nil is True *)
-      dependent destruction h1. cbn. trivial.
-    + (* wt_abs_cons: recurse + forall-part using upVal (which needs ValTy at t1
-         — obtained by applying PEV to the corresponding entry of the bigger pi). *)
-      admit.
-  - (* downPiAppVal: no extra arg (Agda's downVal2 doesn't need ValTy at a1) *)
+    + (* wt_abs_nil *) dependent destruction h1. cbn. trivial.
+    + (* wt_abs_cons *)
+      dependent destruction h1.
+      cbn in PA. destruct PA as [PA_rec PA_forall].
+      cbn. split.
+      * (* Tail recursion: pass the OUTER hPi0/hPi1 (unchanged, since g/b are
+           preserved) and the TAIL h0/h1 (subderivations from dep destr). *)
+        exact (@upPiAppVal _ _ _ _ _ _ _ _ _ _ hPi0 hPi1 h0 h1 LE LEg piEV1 PA_rec).
+      * 
+        move=> P TP VP1.
+        move: (@downVal _ Γ P A0 ui a a0 w w1 LE VP1) => VP.
+        specialize (PA_forall P TP VP).
+        have Vg: valid_fun g. eapply valid_tpi2. eauto with valid.
+        have Vg0: valid_fun g0. eapply valid_tpi2. eauto with valid.
+        have LEt: le t t0.
+        { eapply (@le_fun_mono g g0); eauto. 
+          eauto with valid. } 
+        have WTt0: wt t0 tuniv. eapply wt_ty_tuniv; eauto.
+        have LEMMA : forall n (Γ : Ctx n) P A0 B0 g0 a0 ui t0
+             (hPi1 : wt_pi_fun g0 a0)
+             (piEV1 : PiEdgeVal Γ A0 B0 hPi1)
+             (e0 : app g0 ui = Some t0)
+             (w1 : wt ui a0)
+             (WTt0 : wt t0 tuniv),
+             (typing Γ P A0) -> 
+             (Val Γ P A0 w1) ->
+             Val Γ B0[P..] Core.tuniv WTt0.
+        { clear. 
+          move=> n Γ P A0 B0 g0.
+          all: move=> a0 ui t0 hPi1 PEV APP w1 w2 T1 V1.
+          - admit.
+          - move=> APP w1 WTt0 TO VP.
+            destruct a as [u v].
+            inversion hPi1. subst. 
+            rewrite app_cons_eq in APP.
+        } 
+        have ValT: Val Γ B0[P..] Core.tuniv WTt0.
+        { eapply LEMMA; eauto.  } 
+        eapply upVal. 2: exact LEt. 
+        eapply wt_ty_tuniv; eauto.
+        eauto.
+        eauto.
+
+  - (* downPiAppVal *)
     intros LE LEg PA.
     dependent destruction h1.
     + dependent destruction h0. cbn. trivial.
-    + admit.
+    + dependent destruction h0.
+      cbn in PA. destruct PA as [PA_rec PA_forall].
+      cbn. split.
+      * (* Tail recursion on the wt_abs_fun tails h0, h1 (subderivations). *)
+        exact (@downPiAppVal _ _ _ _ _ _ _ _ _ _ h0 h1 LE LEg PA_rec).
+      * admit.
   - (* upPiAppEq *)
     intros LE LEg PEV PA.
     dependent destruction h0.
     + dependent destruction h1. cbn. trivial.
-    + admit.
+    + dependent destruction h1.
+      cbn in PA. destruct PA as [PA_rec PA_forall].
+      cbn. split.
+      * exact (@upPiAppEq _ _ _ _ _ _ _ _ _ _ hPi0 hPi1 h0 h1 LE LEg PEV PA_rec).
+      * admit.
   - (* downPiAppEq *)
     intros LE LEg PA.
     dependent destruction h1.
     + dependent destruction h0. cbn. trivial.
-    + admit.
+    + dependent destruction h0.
+      cbn in PA. destruct PA as [PA_rec PA_forall].
+      cbn. split.
+      * exact (@downPiAppEq _ _ _ _ _ _ _ _ _ _ h0 h1 LE LEg PA_rec).
+      * admit.
   - (* upPiAppEqVal *)
     intros LE LEg PEV PA.
     dependent destruction h0.
     + dependent destruction h1. cbn. trivial.
-    + admit.
+    + dependent destruction h1.
+      cbn in PA. destruct PA as [PA_rec PA_forall].
+      cbn. split.
+      * exact (@upPiAppEqVal _ _ _ _ _ _ _ _ _ _ _ hPi0 hPi1 h0 h1 LE LEg PEV PA_rec).
+      * admit.
   - (* downPiAppEqVal *)
     intros LE LEg PA.
     dependent destruction h1.
     + dependent destruction h0. cbn. trivial.
-    + admit.
+    + dependent destruction h0.
+      cbn in PA. destruct PA as [PA_rec PA_forall].
+      cbn. split.
+      * exact (@downPiAppEqVal _ _ _ _ _ _ _ _ _ _ _ h0 h1 LE LEg PA_rec).
+      * admit.
   - (* downPiEdgeVal *)
     intros LE LEf PE.
     dependent destruction h0.
@@ -1324,30 +1221,18 @@ Proof.
     dependent destruction h0.
     + cbn. trivial.
     + admit.
-Admitted.
-      
-
-
-(* ---- restrictVal / restrictEqVal: shrink the term-side u ---- *)
-
-(* restrictVal: same a, smaller u' ≤ u *)
-Fixpoint restrictVal {n} (Γ : Ctx n) (M T : Tm n) u u' a
-  (h0 : wt u' a) (h1 : wt u a) {struct h1} :
-  le u' u -> Val Γ M T h1 -> Val Γ M T h0
-with restrictEqVal {n} (Γ : Ctx n) (M N T : Tm n) u u' a
-  (h0 : wt u' a) (h1 : wt u a) {struct h1} :
-  le u' u -> EqVal Γ M N T h1 -> EqVal Γ M N T h0.
-Proof.
-  - admit.
-  - admit.
+  - (* restrictVal: shrink the term-side u (same a, smaller u' ≤ u). *)
+    admit.
+  - (* restrictEqVal *)
+    admit.
 Admitted.
 
 
 (* ---- down on ValTy / EqValTy ---- *)
 
 (* downValTy2 *)
-Lemma downValTy {n} (Γ : Ctx n) (M : Tm n) u0 u1 i
-  (h0 : wt u0 (tuniv i)) (h1 : wt u1 (tuniv i)) :
+Lemma downValTy {n} (Γ : Ctx n) (M : Tm n) u0 u1 
+  (h0 : wt u0 tuniv) (h1 : wt u1 tuniv) :
   le u0 u1 -> ValTy Γ M h1 -> ValTy Γ M h0.
 Proof.
     move=> LE VT1.
@@ -1357,8 +1242,8 @@ Proof.
 Qed.
 
 (* downEqValTy2 *)
-Lemma downEqValTy {n} (Γ : Ctx n) (M N : Tm n) u0 u1 i
-  (h0 : wt u0 (tuniv i)) (h1 : wt u1 (tuniv i)) :
+Lemma downEqValTy {n} (Γ : Ctx n) (M N : Tm n) u0 u1 
+  (h0 : wt u0 tuniv) (h1 : wt u1 tuniv) :
   le u0 u1 -> EqValTy Γ M N h1 -> EqValTy Γ M N h0.
 Proof.
     move=> LE VT1.
@@ -1370,18 +1255,52 @@ Qed.
 
 (* ---- Sup / lub ---- *)
 
+Fixpoint wt_lub u1 u2 a u  
+  (h1: wt u1 a) (h2: wt u2 a) : lub u1 u2 = Some u -> wt u a
+with wt_pi_fun_lub a a0 g g0 e  
+  (w : wt_pi_fun g a) (w0 : wt_pi_fun g0 a0) :
+  lub a a0 = Some e -> 
+  (wt_pi_fun (g ++ g0) e).
+Proof.
+- dependent destruction h1;
+  dependent destruction h2.
+  all: cbn.
+  all: move=> h; inversion h; clear h; subst.
+  all: try solve [econstructor; eauto].
+  + destruct (lub u0 u1) eqn:EQ. inversion H0. subst.
+    eapply wt_succ; eauto.
+    inversion H0.
+  + destruct (compatible_fun g g0) eqn:Cg.
+    destruct (lub a a0) eqn:EQ; inversion H0; subst; clear H0.
+    eapply wt_tpi; eauto. 
+    eapply valid_tpi_intro; eauto with valid.    
+    eapply valid_append. eapply valid_tpi2; eauto.
+    eapply valid_tpi2; eauto. auto.
+    inversion H0.
+  +  destruct (compatible_fun f f0) eqn:EQ; inversion H0; subst; clear H0.
+    eapply wt_abs; eauto. 
+    admit.
+    admit.
+- dependent destruction w;
+  dependent destruction w0.
+  all: cbn.
+  all: move=> h; inversion h; clear h; subst.
+  all: try solve [econstructor; eauto].
+Admitted.
+
+
 (* ValTy2-Sup: if a1 and a2 are universe-members and lub a1 a2 = Some a,
    ValTy at a1 and a2 lifts to ValTy at the lub. *)
-Fixpoint ValTy_Sup {n} (Γ : Ctx n) (T : Tm n) a1 a2 a i
-  (h1 : wt a1 (tuniv i)) (h2 : wt a2 (tuniv i)) (h : wt a (tuniv i)) {struct h}:
+Fixpoint ValTy_Sup {n} (Γ : Ctx n) (T : Tm n) a1 a2 a 
+  (h1 : wt a1 tuniv) (h2 : wt a2 tuniv) (h : wt a tuniv) {struct h}:
   lub a1 a2 = Some a ->
   ValTy Γ T h1 -> ValTy Γ T h2 -> ValTy Γ T h.
 Proof.
 Admitted.
 
 (* EqValTy2-Sup *)
-Lemma EqValTy_Sup {n} (Γ : Ctx n) (M N : Tm n) a1 a2 a i
-  (h1 : wt a1 (tuniv i)) (h2 : wt a2 (tuniv i)) (h : wt a (tuniv i)) :
+Lemma EqValTy_Sup {n} (Γ : Ctx n) (M N : Tm n) a1 a2 a 
+  (h1 : wt a1 tuniv) (h2 : wt a2 tuniv) (h : wt a tuniv) :
   lub a1 a2 = Some a ->
   EqValTy Γ M N h1 -> EqValTy Γ M N h2 -> EqValTy Γ M N h.
 Proof. Admitted.
@@ -1390,11 +1309,11 @@ Proof. Admitted.
 (* ----------------------------------------------------- *)
 
 Fixpoint Val_EqVal_fwd {n} (Γ : Ctx n) (M A : Tm n) u a
-  (h : wt u a) (B : Tm n) i (h' : wt a (tuniv i))
+  (h : wt u a) (B : Tm n)  (h' : wt a tuniv)
   {struct h} :
   Val Γ M A h -> EqValTy Γ A B h' -> Val Γ M B h
 with EqVal_EqVal_fwd {n} (Γ : Ctx n) (M N A : Tm n) u a
-  (h : wt u a) (B : Tm n) i (h' : wt a (tuniv i))
+  (h : wt u a) (B : Tm n)  (h' : wt a tuniv)
   {struct h} :
   EqVal Γ M N A h -> EqValTy Γ A B h' -> EqVal Γ M N B h
 with EqVal_sym {n} (Γ : Ctx n) (M1 M2 A : Tm n) u a (h : wt u a) { struct h } :
@@ -1415,7 +1334,7 @@ Admitted.
 
 
 (* EqValTy2-sym *)
-Lemma EqValTy_sym {n} (Γ : Ctx n) (M N : Tm n) u i (h : wt u (tuniv i)) :
+Lemma EqValTy_sym {n} (Γ : Ctx n) (M N : Tm n) u (h : wt u tuniv) :
   EqValTy Γ M N h -> EqValTy Γ N M h.
 Proof.
   move=>h1. eapply EqVal_EqValTy. eapply EqVal_sym.
@@ -1423,7 +1342,7 @@ Proof.
 Qed.
 
 (* EqValTy2-trans *)
-Lemma EqValTy_trans {n} (Γ : Ctx n) (A B C : Tm n) u i (h : wt u (tuniv i)) :
+Lemma EqValTy_trans {n} (Γ : Ctx n) (A B C : Tm n) u (h : wt u tuniv) :
   EqValTy Γ A B h -> EqValTy Γ B C h -> EqValTy Γ A C h.
 Proof.
   move=> h1 h2.
@@ -1438,12 +1357,12 @@ Qed.
 
    Translation conventions (Agda → Rocq):
      FinMem u a              ≈  wt u a
-     FinMem b UCode          ≈  wt b (tuniv i)         (some i)
+     FinMem b UCode          ≈  wt b tuniv         (some i)
      Coherent u              ≈  valid u                (implicit in wt)
      CoherentFun g           ≈  valid_fun g            (implicit in wt (abs g) ..)
      CoherentFunTail f       ≈  valid_fun f            (implicit in wt (tpi _ f) ..)
      FinMemFun g b f         ≈  wt (abs g) (tpi b f)
-     FinMemAllU f b          ≈  wt (tpi b f) (tuniv i) (codomains in U_i)
+     FinMemAllU f b          ≈  wt (tpi b f) tuniv (codomains in U_i)
      LeCode u v              ≈  le u v
      LeFunCode f g           ≈  le_fun f g
      Comp u v                ≈  compatible u v
@@ -1514,15 +1433,15 @@ Qed.
    ============================================================ *)
 
 (* EqValTy2-headred-expand *)
-Lemma EqValTy_headred_expand {n} (Γ : Ctx n) (M1 M2 M1' M2' : Tm n) u i
-  (h : wt u (tuniv i)) :
+Lemma EqValTy_headred_expand {n} (Γ : Ctx n) (M1 M2 M1' M2' : Tm n) u 
+  (h : wt u tuniv) :
   HeadRed M1' M1 -> HeadRed M2' M2 ->
   EqValTy Γ M1 M2 h -> EqValTy Γ M1' M2' h.
 Proof. Admitted.
 
 (* EqValTy2-headred-contract *)
-Lemma EqValTy_headred_contract {n} (Γ : Ctx n) (M1 M2 M1' M2' : Tm n) u i
-  (h : wt u (tuniv i)) :
+Lemma EqValTy_headred_contract {n} (Γ : Ctx n) (M1 M2 M1' M2' : Tm n) u 
+  (h : wt u tuniv) :
   HeadRed M1 M1' -> HeadRed M2 M2' ->
   EqValTy Γ M1 M2 h -> EqValTy Γ M1' M2' h.
 Proof. Admitted.
@@ -1608,7 +1527,7 @@ Proof. Admitted.
    the mutual Fixpoint block defining upVal / upEqVal / downVal / downEqVal
    above. The signatures there take wt_abs_fun / wt_pi_fun derivations
    directly (the underlying derivations of the wt judgment), instead of
-   wt (abs g) (tpi b f) / wt (tpi b f) (tuniv i) — see the block above
+   wt (abs g) (tpi b f) / wt (tpi b f) tuniv — see the block above
    for the actual statements.
 
    The transport / restrict lemmas below remain as standalone (Admitted)
